Foundation/Modal/Kripke/AxiomH.lean
@@ -76,7 +76,7 @@ lemma isDetourFree_of_validate_axiomH (h : F ⊧ (Axioms.H (.atom 0))) : F.IsDet
   contrapose! h;
   rcases h with ⟨x, u, y, Rxu, Ruy, neux, neuy⟩;
   apply ValidOnFrame.not_of_exists_valuation_world;
-  use λ w _ => w ≠ u, x;
+  use λ _ w => w ≠ u, x;
   simp [Satisfies];
   tauto;
 
