Foundation/Modal/Kripke/AxiomPoint4.lean
@@ -73,9 +73,9 @@ lemma sobocinskiCondition_of_validate_axiomPoint4 (h : F ⊧ (Axioms.Point4 (.at
     contrapose!;
     rintro ⟨x, y, z, nexy, Rxy, Rxz, Rzy⟩;
     apply ValidOnFrame.not_of_exists_valuation_world;
-    suffices ∃ V : Valuation F, ∃ x z, x ≺ z ∧ (∀ w, z ≺ w → V w 0) ∧ V x 0 ∧ ∃ y, x ≺ y ∧ ¬V y 0 by
+    suffices ∃ V : Valuation F, ∃ x z, x ≺ z ∧ (∀ w, z ≺ w → V 0 w) ∧ V 0 x ∧ ∃ y, x ≺ y ∧ ¬V 0 y by
       simpa [Axioms.Point4, Satisfies];
-    use (λ w _ => w = x ∨ z ≺ w), x, z;
+    use (λ _ w => w = x ∨ z ≺ w), x, z;
     refine ⟨?_, ?_, ?_, ?_⟩;
     . assumption;
     . tauto;
