Foundation/Modal/Kripke/Logic/KTB.lean
@@ -66,7 +66,7 @@ instance : Modal.KT ⪱ Modal.KTB := by
     . exact axiomB!;
     . apply Sound.not_provable_of_countermodel (𝓜 := FrameClass.KT);
       apply Kripke.not_validOnFrameClass_of_exists_model_world;
-      let M : Model := ⟨⟨Fin 2, λ x y => x ≤ y⟩, λ w _ => w = 0⟩;
+      let M : Model := ⟨⟨Fin 2, λ x y => x ≤ y⟩, λ _ w => w = 0⟩;
       use M, 0;
       constructor;
       . tauto;
@@ -88,7 +88,7 @@ instance : Modal.KDB ⪱ Modal.KTB := by
     . exact axiomT!;
     . apply Sound.not_provable_of_countermodel (𝓜 := FrameClass.KDB);
       apply Kripke.not_validOnFrameClass_of_exists_model_world;
-      use ⟨⟨Fin 2, λ x y => x ≠ y⟩, λ x _ => x = 1⟩, 0;
+      use ⟨⟨Fin 2, λ x y => x ≠ y⟩, λ _ x => x = 1⟩, 0;
       constructor;
       . refine {
           serial := by
