Foundation/Modal/Kripke/Logic/S4Point2McK.lean
@@ -53,7 +53,7 @@ instance : Modal.S4McK ⪱ Modal.S4Point2McK := by
     . simp;
     . apply Sound.not_provable_of_countermodel (𝓜 := Kripke.FrameClass.S4McK);
       apply Kripke.not_validOnFrameClass_of_exists_model_world;
-      let M : Model := ⟨⟨Fin 3, λ x y => x = 0 ∨ x = y⟩, λ w a => w = 1⟩;
+      let M : Model := ⟨⟨Fin 3, λ x y => x = 0 ∨ x = y⟩, λ a w => w = 1⟩;
       use M, 0;
       constructor
       . exact {
@@ -86,7 +86,7 @@ instance : Modal.S4Point2 ⪱ Modal.S4Point2McK := by
     . simp;
     . apply Sound.not_provable_of_countermodel (𝓜 := Kripke.FrameClass.S4Point2);
       apply Kripke.not_validOnFrameClass_of_exists_model_world;
-      let M : Model := ⟨⟨Fin 2, λ x y => True⟩, λ w _ => w = 0⟩;
+      let M : Model := ⟨⟨Fin 2, λ x y => True⟩, λ _ w => w = 0⟩;
       use M, 0;
       constructor;
       . refine {
