Foundation/Modal/Kripke/Logic/Triv.lean
@@ -91,7 +91,7 @@ instance : Modal.KTc ⪱ Modal.Triv := by
     . simp;
     . apply Sound.not_provable_of_countermodel (𝓜 := Kripke.FrameClass.KTc);
       apply Kripke.not_validOnFrameClass_of_exists_model_world;
-      use ⟨⟨Fin 2, λ x y => False⟩, λ w _ => False⟩, 0;
+      use ⟨⟨Fin 2, λ x y => False⟩, λ _ w => False⟩, 0;
       constructor;
       . refine ⟨by tauto⟩;
       . simp [Satisfies, Semantics.Models];
@@ -108,7 +108,7 @@ instance : Modal.GrzPoint3 ⪱ Modal.Triv := by
     . simp;
     . apply Sound.not_provable_of_countermodel (𝓜 := Kripke.FrameClass.finite_GrzPoint3);
       apply Kripke.not_validOnFrameClass_of_exists_model_world;
-      let M : Model := ⟨⟨Fin 2, λ x y => x ≤ y⟩, (λ w _ => w = 0)⟩;
+      let M : Model := ⟨⟨Fin 2, λ x y => x ≤ y⟩, (λ _ w => w = 0)⟩;
       use M, 0;
       constructor;
       . exact {}
@@ -127,7 +127,7 @@ instance : Modal.S4Point4McK ⪱ Modal.Triv := by
     . simp;
     . apply Sound.not_provable_of_countermodel (𝓜 := Kripke.FrameClass.S4Point4McK);
       apply Kripke.not_validOnFrameClass_of_exists_model_world;
-      let M : Model := ⟨⟨Fin 2, λ x y => x ≤ y⟩, (λ w _ => w = 0)⟩;
+      let M : Model := ⟨⟨Fin 2, λ x y => x ≤ y⟩, (λ _ w => w = 0)⟩;
       use M, 0;
       constructor;
       . exact {
